\section{Sobolev-type inequality}
\label{apdx-sobolev-ineq}

In this section we prove a Sobolev-type inequality analogical to the inequality (7.16) in \cite{BEH}. The presented proof is a simple modification of their proof.
\begin{lemma}
	Let $\psi \in W^{1,2}(\R)$, then for every $a>0$ there exists $b>0$ such that
	\begin{equation}
		\norm{\psi}^{\,n}_{L^\infty(\R)}
		\leq
		a \, \norm{\psi'}^{\,n}_{L^2(\R)} +
		b \, \norm{\psi}^{\,n}_{L^2(\R)}
		\: ,
		\label{sobolev-type-0}
	\end{equation}
	where $n \in \{ 1, 2 \}$.
	\label{lemma-sobolev-type-inequality}
\end{lemma}
\begin{proof}
	We define $\phi := \Fourier \psi$. Since, by definition, $\psi' \in L^2(\R)$ we have $\Fourier \psi' = T_x \Fourier \psi = T_x \phi \in L^2(\R)$, where $T_x$ means the operator of multiplication by the identity function $x \mapsto x$. Next, we utilize the HÃ¶lder inequality to find an estimate of $\lVert\phi\rVert_{L^1}$.
	\begin{equation}
		\norm{\phi}_{L^1}
		\!=
		\norm{\tfrac{1}{x+\i} \, (x+\i) \, \phi(x) }_{L^1}
		\!\leq \underbrace{ \norm{\tfrac{1}{x+\i}}_{L^2} }_{=: \, c}
		\; \norm{(x+\i) \, \phi(x)}_{L^2}
		\leq \,c\, \Big(
			\norm{T_x \, \phi}_{L^2} \!+
			\norm{\phi}_{L^2}
		\Big)
		\: .
		\label{sobolev-type-1}
	\end{equation}
	Since $\phi \in L^1$, it follows that $\psi \in L^\infty$ and
	\begin{equation}
		\norm{\psi}_{L^\infty}
		\leq \frac{1}{\sqrt{2\pi}} \,
		\norm{\phi}_{L^1}
		\: .
		\label{sobolev-type-2}
	\end{equation}
	We introduce a scaled function $\phi_r(x) := r \, \phi(r x)$. Scaling changes the norms in the following way:
	\begin{gather*}
		\norm{\phi_r}_{L^2}^{\,2}
		= r \, \norm{\phi}_{L^2}^{\,2}
		\: ,
		\qquad
		\norm{T_x \phi_r}_{L^2}^{\,2}
		= \frac{1}{r} \, \norm{T_x}_{L^2}^{\,2}
		\: .
	\end{gather*}
	By substituting $\phi \mapsto \phi_r$ in \eqref{sobolev-type-1} and combining with \eqref{sobolev-type-2}, we get
	\begin{gather*}
		\norm{\psi}_{L^\infty}
		\leq
		c \, \sqrt{r} \, \norm{T_x \, \phi}_{L^2} \!+
		\frac{c}{\sqrt{r}} \, \norm{\phi}_{L^2}
		=
		c \, \sqrt{r} \, \norm{\psi'}_{L^2} \!+
		\frac{c}{\sqrt{r}} \, \norm{\psi}_{L^2}
		\: .
	\end{gather*}
	Choosing $r = a^2/c^2$, we have proven the inequality \eqref{sobolev-type-0} for $n=1$.

	To prove $n=2$, we start with the case $n=1$ and square both sides of the inequality.
	\begin{gather*}
		\\[-1.7\baselineskip]
		\norm{\psi}_{L^\infty}
		\leq
		a \, \norm{\psi'}_{L^2}
		+ b \, \norm{\psi}_{L^2}
		\\[5pt]
		\norm{\psi}_{L^\infty}^{\,2}
		\leq
		a \, \norm{\psi'}_{L^2}^{\,2}
		+ 2ab \, \norm{\psi'}_{L^2} \, \norm{\psi}_{L^2}
		+ b \, \norm{\psi}_{L^2}^{\,2}
		\leq
		2a \, \norm{\psi'}_{L^2}^{\,2}
		+ 2b \, \norm{\psi}_{L^2}^{\,2}
	\end{gather*}
	In the last step we have used the fact, that
	\begin{equation*}
		0 \leq
		\big( a\, \norm{\psi'}_{L^2} - b\, \norm{\psi}_{L^2} \big)^2
		\quad \Leftrightarrow \quad
		2ab \, \norm{\psi'}_{L^2} \, \norm{\psi}_{L^2}
		\leq
		a \, \norm{\psi'}_{L^2}^{\,2}
		+ b \, \norm{\psi}_{L^2}^{\,2}
		\: .
	\end{equation*}
	Finally, substituting $2a^2 \mapsto a$ and $2b^2 \mapsto b$, we have proven the inequality for~${n=2}$.
\end{proof}